src/Parsers/Refinement/SharpenedExpressionPlus.v
@@ -1,16 +1,6 @@
 (** Sharpened ADT for an expression grammar with + *)
-Require Import Coq.Init.Wf Coq.Arith.Wf_nat.
-Require Import Coq.Lists.List.
-Require Import Coq.Numbers.Natural.Peano.NPeano.
 Require Import Fiat.Parsers.Refinement.Tactics.
 Require Import Fiat.Parsers.Grammars.ExpressionNumPlus.
-Require Import Fiat.Computation.Refinements.General.
-Require Import Fiat.Parsers.StringLike.Properties.
-Require Import Fiat.Parsers.StringLike.String.
-Require Import Fiat.Common.
-Require Import Fiat.Common.Wf.
-Require Import Fiat.Parsers.Splitters.RDPList.
-Require Import Fiat.Parsers.BaseTypes.
 Require Import Fiat.Parsers.Refinement.FixedLengthLemmas.
 Require Import Fiat.Parsers.Refinement.DisjointRules.
 Require Import Fiat.Parsers.ExtrOcamlParsers. (* for simpl rules for [find_first_char_such_that] *)
@@ -18,7 +8,7 @@ Require Import Fiat.Parsers.ExtrOcamlParsers. (* for simpl rules for [find_first
 Set Implicit Arguments.
 
 Section IndexedImpl.
-Typeclasses Opaque If_Then_Else.
+
   Lemma ComputationalSplitter'
   : FullySharpened (string_spec plus_expr_grammar).
   Proof.
@@ -39,24 +29,22 @@ Typeclasses Opaque If_Then_Else.
   Lemma ComputationalSplitter
   : FullySharpened (string_spec plus_expr_grammar).
   Proof.
-    let impl := (eval simpl in (projT1 ComputationalSplitter')) in
+    let impl := (splitter_red (projT1 ComputationalSplitter')) in
     refine (existT _ impl _).
     abstract (exact (projT2 ComputationalSplitter')).
   Defined.
 
 End IndexedImpl.
 
-Global Arguments ComputationalSplitter / .
-
 Require Import Fiat.Parsers.ParserFromParserADT.
 Require Import Fiat.Parsers.ExtrOcamlParsers.
 Import Fiat.Parsers.ExtrOcamlParsers.HideProofs.
 
-(* Ben : Taking too long to run; commenting so I can debug build.
-
-Time Definition paren_expr_parser (str : String.string) : bool
-  := Eval simpl in has_parse (parser ComputationalSplitter) str.
+Definition paren_expr_parser (str : String.string) : bool.
+Proof.
+  Time make_parser ComputationalSplitter. (* 15 s *)
+Defined.
 
 Print paren_expr_parser.
 
-Recursive Extraction paren_expr_parser. *)
+Recursive Extraction paren_expr_parser.
